\documentclass{article}

\usepackage{amssymb}
\usepackage[fleqn]{amsmath}
\usepackage[utf8]{inputenc}
\usepackage{varwidth}

\title{Aufgabe 1}
\date{}

\begin{document}

\maketitle

\section{}
\subsection{}
$f: M \rightarrow \mathbb{R}$\\
\noindent
\begin{align*}
||f||_1 := \sum_{x \in M}{|f(x)|}
\end{align*}\\
\[||f||_\infty := \sup_{x \in M} ||f(x)||_\mathbb{R} = \sup \{|f(x)| : x \in M\}\]\\
\\
f(0) = 2, f(1) = -4, f(2) = 8, f(3) = -4\\
g(0) = 5, g(1) = 1, g(2) = 7, g(3) = -3\\
\\
\[||f-g||_1 = \sum_{x \in M}{|f(x) - g(x)|}\]\\
= $| 2-5| + |-4 -1| + |8-7| + |-4 - (-3)|$\\
= $ 3 + 5 + 1 + 1$\\
= 10\\
\\
\[||f-g||_\infty = \sup_{x \in M} ||f(x) - g(x)||_\mathbb{R} = \sup \{|f(x) - g(x)| : x\in M\}\]\\
\\
$|f(0) - g(0)| = |2 - 5| = 3$\\
$|f(1) - g(1)| = |-4 - 1| = 5$\\
$|f(2) - g(2)| = |8 - 7| = 1$ \\
$|f(3) - g(3)| = |-4 - (-3)| = 1$\\
\[\rightarrow \sup_{x \in M} ||f(x) - g(x)||_\mathbb{R} = 5\]\\
\\
\subsection{}
\subsubsection{Positive definite}
Assumption: $||f||_1 = 0 \Rightarrow f = 0$\\
\\
Proof:\\
\[||f||_1 =  0 \Leftrightarrow \sum_{x \in M}{|f(x)|} = 0\] \\
\[ \Rightarrow \sum_{x \in M} {|f(x)|} = 0\] \\
$ \Rightarrow| f(0)| + |f(1)| + ... + |f(x)| = 0$ \\
$ \Rightarrow f(x) = 0~\forall x$ \\
$\Rightarrow f = 0$

\subsubsection{Homogeneous}
Assumption: $||\alpha f||_1 = |\alpha|~||f||_1, \alpha \in \mathbb{R}$\\
\\
Proof:\\
\[||\alpha f||_1 := \sum_{x \in M}{|\alpha|~|f(x)|}\]\\
\[\Rightarrow \sum_{x \in M}{|\alpha|~|f(x)|} = |\alpha| \cdot |f(0)| + |\alpha| \cdot |f(1)| + ... + |\alpha| \cdot |f(x)\] \\
$\Rightarrow |\alpha| \cdot ( |f(0)| + |f(1)| + ... + |f(x)|)$ \\
\[\Rightarrow |\alpha| \cdot \sum_{x \in M}{ |f(x)|}\] \\
$\Rightarrow |\alpha|~||f||_1$\\
Since $\alpha$ has to be positive for our usage, we can write $\alpha$ instead of $|\alpha|$ and thus gain: $\alpha ||f||_1$
\newpage
\subsubsection{Triangle inequality}
Assumption: $||f + g||_1 \leq ||f||_1 + ||g||_1$\\
\\
Proof: \\
\[ \Rightarrow \sum_{x \in M}{|f(x) + g(x)|} \leq \sum_{x \in M} {|f(x)|} + \sum_{x \in M}{|g(x)} \] \\
\\
\[ \Rightarrow \sum_{x \in M}{-f(x)} \leq \sum_{x \in M}{|f(x)|} \]\\
and \\
\[ \sum_{x \in M} {-g(x)} \leq \sum_{x \in M}{|g(x)|}\] \\
\\
and \\
\[ \sum_{x \in M}{f(x)} \leq \sum_{x \in M}{|f(x)|} \] \\
and \\
\[ \sum_{x \in M}{g(x)} \leq \sum_{x \in M}{|g(x)|} \] \\
\\
\[ \Rightarrow \sum_{x \in M} {-f(x) + g(x) } \leq \sum_{x \in M}{|f(x) + g(x)|} \leq \sum_{x \in M} {|f(x)| + g(x) } \leq \sum_{x \in M} {|f(x)| + |g(x)| } = \sum_{x \in M} {|f(x)|} + \sum_{x \in M} {|g(x)|} \\
\\
and \\
\[ \Rightarrow \sum_{x \in M} {f(x) + (-g(x)) } \leq \sum_{x \in M}{|f(x) + g(x)|} \leq \sum_{x \in M} {f(x) + |g(x)| } \leq \sum_{x \in M} {|f(x)| + |g(x)| } = \sum_{x \in M} {|f(x)|} + \sum_{x \in M} {|g(x)|} \\


\end{document}